Define and prove normal substitution

Defs.thy
@@ -2,26 +2,31 @@ theory Defs
 imports Main "Nominal2.Nominal2" "HOL-Eisbach.Eisbach"
 begin
 
-atom_decl "name"
+atom_decl "var"
+atom_decl "tyvar"
+
 nominal_datatype "\<tau>" =
   TyUnit
- | TyArrow "\<tau>" "\<tau>"  ("_ \<rightarrow> _" 50)
+  | TyVar "tyvar"
+  | TyArrow "\<tau>" "\<tau>"  ("_ \<rightarrow> _" 50)
+  | TyForall a::"tyvar" t::"\<tau>" binds a in t ("\<forall> _ . _" 50)
 
 nominal_datatype "term" =
-   Var "name"
- | Lam x::"name" "\<tau>" e::"term" binds x in e  ("\<lambda> _ : _ . _" 50)
+   Var "var"
+ | Lam x::"var" "\<tau>" e::"term" binds x in e  ("\<lambda> _ : _ . _" 50)
+ | TyLam a::"tyvar" e::"term" binds a in e ("\<Lambda> _ . _" 50)
  | App "term" "term"
  | Unit
- | Let x::"name" "term" e2::"term" binds x in e2
+ | Let x::"var" "term" e2::"term" binds x in e2
 
-type_synonym "\<Gamma>" = "(name * \<tau>) list"
+type_synonym "\<Gamma>" = "(var * \<tau>) list"
 
 declare term.fv_defs[simp]
 
-lemma no_vars_in_ty[simp]: "atom x \<sharp> (ty :: \<tau>)"
+lemma no_vars_in_ty[simp]: "atom (x :: var) \<sharp> (ty :: \<tau>)"
   by (induction ty rule: \<tau>.induct) auto
 
-nominal_function isin :: "name * \<tau> \<Rightarrow> \<Gamma> \<Rightarrow> bool" (infixr "\<in>" 80) where
+(*nominal_function isin :: "var * \<tau> \<Rightarrow> \<Gamma> \<Rightarrow> bool" (infixr "\<in>" 80) where
   "isin _ [] = False"
 | "isin (x, t) ((y, t')#xs) = (if x = y then t = t' else isin (x, t) xs)"
        apply (all_trivials)
@@ -29,51 +34,130 @@ nominal_function isin :: "name * \<tau> \<Rightarrow> \<Gamma> \<Rightarrow> boo
      apply (metis list.exhaust old.prod.exhaust)
     apply simp
   done
-nominal_termination (eqvt) by lexicographic_order
+nominal_termination (eqvt) by lexicographic_order*)
 
 (** subrules *)
 nominal_function
-is_v_of_e :: "term => bool"
+is_value :: "term => bool"
 where
-"is_v_of_e (Var x) = (False)"
-| "is_v_of_e (\<lambda> x : \<tau> . e) = ((True))"
-| "is_v_of_e (App e1 e2) = (False)"
-| "is_v_of_e Unit = ((True))"
-| "is_v_of_e (Let x e1 e2) = (False)"
-  apply (all_trivials)
-  apply (simp add: eqvt_def is_v_of_e_graph_aux_def)
+"is_value (Var x) = False"
+| "is_value (\<lambda> x : \<tau> . e) = True"
+| "is_value (\<Lambda> a . e) = True"
+| "is_value (App e1 e2) = False"
+| "is_value Unit = True"
+| "is_value (Let x e1 e2) = False"
+  apply (auto simp: eqvt_def is_value_graph_aux_def)
   using term.exhaust by blast
-nominal_termination (eqvt)
-  by lexicographic_order
+nominal_termination (eqvt) by lexicographic_order
 
-method pat_comp_aux =
-  (match premises in
-    "x = (_ :: term) \<Longrightarrow> _" for x \<Rightarrow> \<open>rule term.strong_exhaust [where y = x and c = x]\<close>
-  \<bar> "x = (Var _, _) \<Longrightarrow> _" for x :: "_ :: fs" \<Rightarrow>
-    \<open>rule term.strong_exhaust [where y = "fst x" and c = x]\<close>
-  \<bar> "x = (_, Var _) \<Longrightarrow> _" for x :: "_ :: fs" \<Rightarrow>
-    \<open>rule term.strong_exhaust [where y = "snd x" and c = x]\<close>
-  \<bar> "x = (_, _, Var _) \<Longrightarrow> _" for x :: "_ :: fs" \<Rightarrow>
-    \<open>rule term.strong_exhaust [where y = "snd (snd x)" and c = x]\<close>)
+lemma Abs_lst_rename: "\<lbrakk> atom c \<sharp> e ; sort_of (atom c) = sort_of (atom a) \<rbrakk> \<Longrightarrow> [[atom a]]lst. e = [[atom c]]lst. (a \<leftrightarrow> c) \<bullet> e"
+proof -
+  assume a: "atom c \<sharp> e" and a2: "sort_of (atom c) = sort_of (atom a)"
+  then have 1: "atom c \<notin> supp e - set [atom a]" by (simp add: fresh_def)
+  have 2: "atom a \<notin> supp e - set [atom a]" by simp
+  show ?thesis using Abs_swap2[OF 2 1] by (simp add: a2 flip_def)
+qed
+
+lemma Abs_lst_rename_both:
+"\<lbrakk> atom c \<sharp> (y, e::'e::fs, y', e'::'e::fs) ; sort_of (atom c) = sort_of (atom y) ; sort_of (atom c) = sort_of (atom y') ; ([[atom y]]lst. e) = ([[atom y']]lst. e') \<rbrakk> \<Longrightarrow>
+  (y \<leftrightarrow> c) \<bullet> e = (y' \<leftrightarrow> c) \<bullet> e'"
+proof -
+  assume a: "atom c \<sharp> (y, e, y', e')" "sort_of (atom c) = sort_of (atom y)" "sort_of (atom c) = sort_of (atom y')" "([[atom y]]lst. e) = ([[atom y']]lst. e')"
+  then have "(y \<leftrightarrow> c) \<bullet> ([[atom y]]lst. e) = (y' \<leftrightarrow> c) \<bullet> ([[atom y']]lst. e')"
+    by (smt Abs_lst_rename Cons_eqvt Nil_eqvt flip_def fresh_PairD(1) fresh_PairD(2) permute_Abs_lst swap_atom_simps(1))
+  then have "([[atom c]]lst. (y \<leftrightarrow> c) \<bullet> e) = ([[atom c]]lst. (y' \<leftrightarrow> c) \<bullet> e')" using Abs_lst_rename a(2) a(3) by auto
+  then show ?thesis using Abs1_eq(3) by blast
+qed
+
+lemma eqvt_at_deep: "\<lbrakk> atom a \<sharp> (x, e) ; atom c \<sharp> (x, e) ; eqvt_at f (e, x, e2) \<rbrakk> \<Longrightarrow> (a \<leftrightarrow> c) \<bullet> f (e, x, e2) = f (e, x, (a \<leftrightarrow> c) \<bullet> e2)"
+proof -
+  assume a: "atom a \<sharp> (x, e)" "atom c \<sharp> (x, e)" "eqvt_at f (e, x, e2)"
+
+  have 1: "(a \<leftrightarrow> c) \<bullet> f (e, x, e2) = f ((a \<leftrightarrow> c) \<bullet> (e, x, e2))" using a(3) eqvt_at_def by blast
+  have 2: "(a \<leftrightarrow> c) \<bullet> (e, x, e2) = (e, x, (a \<leftrightarrow> c) \<bullet> e2)" using a(1) a(2) fresh_Pair flip_fresh_fresh by fastforce
+
+  show ?thesis using 1 2 by argo
+qed
+
+lemma Abs_lst_rename_deep: "\<lbrakk> atom c \<sharp> (f (e, x, e2), x, e) ; atom a \<sharp> (x, e) ; sort_of (atom c) = sort_of (atom a) ; eqvt_at f (e, x, e2) \<rbrakk> \<Longrightarrow> [[atom a]]lst. f (e, x, e2) = [[atom c]]lst. f (e, x, (a \<leftrightarrow> c) \<bullet> e2)"
+proof -
+  assume a: "atom c \<sharp> (f (e, x, e2), x, e)" "atom a \<sharp> (x, e)" "sort_of (atom c) = sort_of (atom a)" "eqvt_at f (e, x, e2)"
+
+  have 1: "[[atom a]]lst. f (e, x, e2) = [[atom c]]lst. (a \<leftrightarrow> c) \<bullet> f (e, x, e2)" using Abs_lst_rename[OF _ a(3)] a(1) fresh_Pair by blast
+  have 2: "(a \<leftrightarrow> c) \<bullet> f (e, x, e2) = f (e, x, (a \<leftrightarrow> c) \<bullet> e2)" using eqvt_at_deep[OF a(2) _ a(4)] a(1) fresh_Pair by blast
+
+  show ?thesis using 1 2 by argo
+qed
 
 (** substitutions *)
 nominal_function
-subst_term :: "term => name => term => term"
+subst_term :: "term => var => term => term"
 where
-"subst_term e_5 x5 (Var x) = ((if x=x5 then e_5 else (Var x)))"
-| "atom x \<sharp> (x5, e_5) \<Longrightarrow> subst_term e_5 x5 (\<lambda> x : \<tau> . e) = (Lam x \<tau> (subst_term e_5 x5 e))"
-| "subst_term e_5 x5 (App e1 e2) = (App (subst_term e_5 x5 e1) (subst_term e_5 x5 e2))"
-| "subst_term e_5 x5 Unit = (Unit )"
-| "atom x \<sharp> (x5, e_5) \<Longrightarrow> subst_term e_5 x5 (Let x e1 e2) = (Let x (subst_term e_5 x5 e1) (subst_term e_5 x5 e2))"
-                   apply (all_trivials)
-        apply (simp add: eqvt_def subst_term_graph_aux_def)
-      apply(pat_comp_aux)
-          apply(auto simp: fresh_star_def fresh_Pair)
-     apply blast
-    apply blast
-   apply (auto simp: eqvt_at_def)
-   apply (metis flip_fresh_fresh)+
-  done
+"subst_term e x (Var y) = (if x=y then e else Var y)"
+| "atom y \<sharp> (x, e) \<Longrightarrow> subst_term e x (\<lambda> y : \<tau> . e2) = (Lam y \<tau> (subst_term e x e2))"
+| "atom y \<sharp> (x, e) \<Longrightarrow> subst_term e x (\<Lambda> y . e2) = (\<Lambda> y . subst_term e x e2)"
+| "subst_term e x (App e1 e2) = (App (subst_term e x e1) (subst_term e x e2))"
+| "subst_term _ _ Unit = Unit"
+| "atom y \<sharp> (x, e) \<Longrightarrow> subst_term e x (Let y e1 e2) = (Let y (subst_term e x e1) (subst_term e x e2))"
+proof goal_cases
+  case (3 P x)
+  then obtain e y t where P: "x = (e, y, t)" by (metis prod.exhaust)
+  then show ?case
+    apply (cases t rule: term.strong_exhaust[of _ _ "(y, e)"])
+         apply (auto simp: 3)
+    using 3(2) 3(3) 3(6) P fresh_star_def by blast+
+next
+  case (10 y x e \<tau> e2 y' x' e' \<tau>' e2')
+
+  obtain c::var where "atom c \<sharp> (y, y',  e, x, e', x', e2, e2', subst_term_sumC (e, x, e2), subst_term_sumC (e', x', e2'))" using obtain_fresh by blast
+  then have c: "atom c \<sharp> (subst_term_sumC (e, x, e2), x, e)" "atom c \<sharp> (subst_term_sumC (e', x', e2'), x', e')" "atom c \<sharp> (y, e2, y', e2')" using fresh_Pair by fastforce+
+
+  have sort_same_y: "sort_of (atom c) = sort_of (atom y)" by simp
+  have sort_same_y': "sort_of (atom c) = sort_of (atom y')" by simp
+
+  have 1: "(\<lambda> y : \<tau> . subst_term_sumC (e, x, e2)) = (\<lambda> c : \<tau> . subst_term_sumC (e, x, (y \<leftrightarrow> c) \<bullet> e2))"
+    using Abs_lst_rename_deep[OF c(1) 10(5) sort_same_y 10(1)] term.eq_iff(2) by blast
+  have 2: "(\<lambda> y' : \<tau>' . subst_term_sumC (e', x', e2')) = (\<lambda> c : \<tau> . subst_term_sumC (e, x, (y' \<leftrightarrow> c) \<bullet> e2'))"
+    using Abs_lst_rename_deep[OF c(2) 10(6) sort_same_y' 10(2)] term.eq_iff(2) 10(7) by auto
+  have 3: "(y \<leftrightarrow> c) \<bullet> e2 = (y' \<leftrightarrow> c) \<bullet> e2'" using Abs_lst_rename_both[OF c(3) sort_same_y sort_same_y'] 10(7) by force
+
+  show ?case using 1 2 3 by argo
+next
+  case (15 y x e e2 y' x' e' e2')
+  
+  obtain c::tyvar where "atom c \<sharp> (y, y',  e, x, e', x', e2, e2', subst_term_sumC (e, x, e2), subst_term_sumC (e', x', e2'))" using obtain_fresh by blast
+  then have c: "atom c \<sharp> (subst_term_sumC (e, x, e2), x, e)" "atom c \<sharp> (subst_term_sumC (e', x', e2'), x', e')" "atom c \<sharp> (y, e2, y', e2')" using fresh_Pair by fastforce+
+
+  have sort_same_y: "sort_of (atom c) = sort_of (atom y)" by simp
+  have sort_same_y': "sort_of (atom c) = sort_of (atom y')" by simp
+
+  have 1: "(\<Lambda> y . subst_term_sumC (e, x, e2)) = (\<Lambda> c . subst_term_sumC (e, x, (y \<leftrightarrow> c) \<bullet> e2))"
+    using Abs_lst_rename_deep[OF c(1) 15(5) sort_same_y 15(1)] term.eq_iff(3) by presburger
+  have 2: "(\<Lambda> y' . subst_term_sumC (e', x', e2')) = (\<Lambda> c . subst_term_sumC (e, x, (y' \<leftrightarrow> c) \<bullet> e2'))"
+    using Abs_lst_rename_deep[OF c(2) 15(6) sort_same_y' 15(2)] term.eq_iff(3) 15(7) by auto
+  have 3: "(y \<leftrightarrow> c) \<bullet> e2 = (y' \<leftrightarrow> c) \<bullet> e2'" using Abs_lst_rename_both[OF c(3) sort_same_y sort_same_y'] 15(7) by force
+
+  show ?case using 1 2 3 by argo
+next
+  case (24 y x e e1 e2 y' x' e' e1' e2')
+
+  obtain c::var where "atom c \<sharp> (y, y',  e, x, e', x', e2, e2', subst_term_sumC (e, x, e2), subst_term_sumC (e', x', e2'))" using obtain_fresh by blast
+  then have c: "atom c \<sharp> (subst_term_sumC (e, x, e2), x, e)" "atom c \<sharp> (subst_term_sumC (e', x', e2'), x', e')" "atom c \<sharp> (y, e2, y', e2')" using fresh_Pair by fastforce+
+
+  have sort_same_y: "sort_of (atom c) = sort_of (atom y)" by simp
+  have sort_same_y': "sort_of (atom c) = sort_of (atom y')" by simp
+
+  let ?e1 = "subst_term_sumC (e, x, e1)"
+  let ?e1' = "subst_term_sumC (e', x', e1')"
+  have 0: "?e1 = ?e1'" using 24 by simp
+  have 1: "Let y ?e1 (subst_term_sumC (e, x, e2)) = Let c ?e1 (subst_term_sumC (e, x, (y \<leftrightarrow> c) \<bullet> e2))"
+    using Abs_lst_rename_deep[OF c(1) 24(9) sort_same_y 24(2)] 0 term.eq_iff(6) by blast
+  have 2: "Let y' ?e1' (subst_term_sumC (e', x', e2')) = Let c ?e1 (subst_term_sumC (e, x, (y' \<leftrightarrow> c) \<bullet> e2'))"
+    using Abs_lst_rename_deep[OF c(2) 24(10) sort_same_y' 24(4)] 0 term.eq_iff(6) 24(11) by auto
+  have 3: "(y \<leftrightarrow> c) \<bullet> e2 = (y' \<leftrightarrow> c) \<bullet> e2'" using Abs_lst_rename_both[OF c(3) sort_same_y sort_same_y'] 24(11) by force
+
+  show ?case using 1 2 3 by argo
+qed (auto simp: eqvt_def subst_term_graph_aux_def)
 nominal_termination (eqvt) by lexicographic_order
 
 lemma fresh_subst_term: "\<lbrakk> atom z \<sharp> s ; z = y \<or> atom z \<sharp> t \<rbrakk> \<Longrightarrow> atom z \<sharp> subst_term s y t"
@@ -122,17 +206,17 @@ where
 
 | (* defn Step *)
 
-ST_BetaI: "\<lbrakk>is_v_of_e v\<rbrakk> \<Longrightarrow>
+ST_BetaI: "\<lbrakk>is_value v\<rbrakk> \<Longrightarrow>
 ((App  (\<lambda> x : \<tau> . e)  v) \<longrightarrow>  subst_term  v   x   e )"
 
 | ST_AppI: "\<lbrakk>(e1 \<longrightarrow> e2)\<rbrakk> \<Longrightarrow>
 ((App e1 e) \<longrightarrow> (App e2 e))"
 
-| ST_App2I: "\<lbrakk>is_v_of_e v ;
+| ST_App2I: "\<lbrakk>is_value v ;
 (e1 \<longrightarrow> e2)\<rbrakk> \<Longrightarrow>
 ((App v e1) \<longrightarrow> (App v e2))"
 
-| ST_SubstI: "\<lbrakk>is_v_of_e v\<rbrakk> \<Longrightarrow>
+| ST_SubstI: "\<lbrakk>is_value v\<rbrakk> \<Longrightarrow>
 ((Let x v e) \<longrightarrow>  subst_term  v   x   e )"
 
 | ST_LetI: "\<lbrakk>(e1 \<longrightarrow> e2)\<rbrakk> \<Longrightarrow>
